Sketching SGX memory

examples/sgx/FStar.STX.fst
@@ -6,10 +6,10 @@ open FStar.Heap
 
    If this were using the Dm4Free construction, we would have written the monad as:
 
-   STX (a:Type) = h0:heap                 //the input state
-		-> send_failed:bool       //an input flag, recording whether or not a send has failed so far
-		-> Tot (option (a * heap) //the output state is an optional pair, because throwing an exception discards (and resets) the state
-		        * bool)           //the output flag, recording whether this computation has a failed send
+   STX (a:Type) = h0:sgxmem		//the input state
+		-> rw_failed:bool       //an input flag, recording whether or not a read/write has failed so far
+		-> Tot (option (a * sgxmem) //the output state is an optional pair, because throwing an exception discards (and resets) the state
+		        * bool)           //the output flag, recording whether this computation has a failed read/write
 
    with
 
@@ -22,21 +22,12 @@ open FStar.Heap
 	 | None, b1 -> None, b1 //if the first computation throws, the state is gone, but the flag remains
 	 | Some (x, h1), b1 -> g x h1 b1  //otherwise, we run the second computation with the new state and flag
 
-
-  Much of what follows is this basic idea, but it's a bit convoluted
-  because of the WP style. We should make this work with Dm4Free so
-  that we can really write what's above instead of the verbose stuff
-  that follows.
-
-  One wrinkle is that I define everything first generically over the
-  type of the state, and then instantiate the state to FStar.Heap.heap.
-  That should allow us to plug in whatever memory model you like, later.
 *)
 
 (* You can mostly skip reading from here ...
    <skip> *)
 let stx_pre_h  (h:Type)           = h                //input state is pair of the state h 
-				  -> bool             //and a flag recording the status of the last send
+				  -> bool             //and a flag recording the status of the last read/write
 				  -> GTot Type0
 let stx_post_h (h:Type) (a:Type)  = option (a * h)   //an exceptional result and final state
 				  -> bool             //pair of final state and output flag
@@ -44,17 +35,17 @@ let stx_post_h (h:Type) (a:Type)  = option (a * h)   //an exceptional result and
 let stx_wp_h   (h:Type) (a:Type)  = stx_post_h h a 
 				  -> Tot (est_pre_h h)
 
-inline let stx_ite_wp (heap:Type) (a:Type)
-                      (wp:est_wp_h heap a)
-                      (post:est_post_h heap a) (h0:heap) (b:bool) =
-    forall (k:est_post_h heap a).
-       (forall (x:option (a * heap)) (b:bool).{:pattern (guard_free (k x b))} k x b <==> post x b)
+inline let stx_ite_wp (sgxmem:Type) (a:Type)
+                      (wp:stx_wp_h sgxmem a)
+                      (post:stx_post_h sgxmem a) (h0:sgxmem) (b:bool) =
+    forall (k:stx_post_h sgxmem a).
+       (forall (x:option (a * sgxmem)) (b:bool).{:pattern (guard_free (k x b))} k x b <==> post x b)
        ==> wp k h0 b
-inline let stx_return  (heap:Type) (a:Type) (x:a) (p:est_post_h heap a) (h0:heap) (b:bool)= p (Some (x, h0)) b
-inline let stx_bind_wp (heap:Type) (r1:range) (a:Type) (b:Type)
-                       (wp1:est_wp_h heap a)
-                       (wp2:(a -> GTot (est_wp_h heap b)))
-                       (p:est_post_h heap b) (h0:heap) (b0:bool) : GTot Type0 =
+inline let stx_return  (sgxmem:Type) (a:Type) (x:a) (p:stx_post_h sgxmem a) (h0:sgxmem) (b:bool)= p (Some (x, h0)) b
+inline let stx_bind_wp (sgxmem:Type) (r1:range) (a:Type) (b:Type)
+                       (wp1:stx_wp_h sgxmem a)
+                       (wp2:(a -> GTot (est_wp_h sgxmem b)))
+                       (p:stx_post_h sgxmem b) (h0:sgxmem) (b0:bool) : GTot Type0 =
    labeled r1 "push" unit
    /\ wp1 (fun ra b1 ->
        labeled r1 "pop" unit
@@ -62,73 +53,80 @@ inline let stx_bind_wp (heap:Type) (r1:range) (a:Type) (b:Type)
 	    | None -> p None b1 //if the 1st computation throws, then we don't run the 2nd one
 	    | Some (x, h1) -> wp2 x p h1 b1))
      h0 b0
-inline let stx_if_then_else (heap:Type) (a:Type) (p:Type)
-                             (wp_then:est_wp_h heap a) (wp_else:est_wp_h heap a)
-                             (post:est_post_h heap a) (h0:heap) (b:bool) =
+inline let stx_if_then_else (sgxmem:Type) (a:Type) (p:Type)
+                             (wp_then:stx_wp_h sgxmem a) (wp_else:stx_wp_h sgxmem a)
+                             (post:stx_post_h sgxmem a) (h0:sgxmem) (b:bool) =
    l_ITE p
        (wp_then post h0 b)
        (wp_else post h0 b)
-inline let stx_stronger (heap:Type) (a:Type) (wp1:est_wp_h heap a)
-                        (wp2:est_wp_h heap a) =
-    (forall (p:est_post_h heap a) (h:heap) (b:bool). wp1 p h b ==> wp2 p h b)
+inline let stx_stronger (sgxmem:Type) (a:Type) (wp1:stx_wp_h sgxmem a)
+                        (wp2:stx_wp_h sgxmem a) =
+    (forall (p:stx_post_h sgxmem a) (h:sgxmem) (b:bool). wp1 p h b ==> wp2 p h b)
 
-inline let stx_close_wp (heap:Type) (a:Type) (b:Type)
-                        (wp:(b -> GTot (est_wp_h heap a)))
-                        (p:est_post_h heap a) (h:heap) (f:bool) =
+inline let stx_close_wp (sgxmem:Type) (a:Type) (b:Type)
+                        (wp:(b -> GTot (est_wp_h sgxmem a)))
+                        (p:stx_post_h sgxmem a) (h:sgxmem) (f:bool) =
     (forall (b:b). wp b p h f)
-inline let stx_assert_p (heap:Type) (a:Type) (p:Type)
-                        (wp:est_wp_h heap a) (q:est_post_h heap a) (h:heap) (b:bool) =
+inline let stx_assert_p (sgxmem:Type) (a:Type) (p:Type)
+                        (wp:stx_wp_h sgxmem a) (q:stx_post_h sgxmem a) (h:sgxmem) (b:bool) =
     p /\ wp q h b
-inline let stx_assume_p (heap:Type) (a:Type) (p:Type)
-                         (wp:est_wp_h heap a) (q:est_post_h heap a) (h:heap) (b:bool) =
+inline let stx_assume_p (sgxmem:Type) (a:Type) (p:Type)
+                         (wp:stx_wp_h sgxmem a) (q:stx_post_h sgxmem a) (h:sgxmem) (b:bool) =
     p ==> wp q h b
-inline let stx_null_wp (heap:Type) (a:Type)
-                       (p:est_post_h heap a) (h0:heap) (b:bool) =
-    (forall (a:option (a * heap)) (b1:bool). p a b1)
-inline let stx_trivial (heap:Type) (a:Type) (wp:est_wp_h heap a) =
-    (forall (h0:heap) (b:bool). wp (fun r b -> True) h0 b)
+inline let stx_null_wp (sgxmem:Type) (a:Type)
+                       (p:stx_post_h sgxmem a) (h0:sgxmem) (b:bool) =
+    (forall (a:option (a * sgxmem)) (b1:bool). p a b1)
+inline let stx_trivial (sgxmem:Type) (a:Type) (wp:stx_wp_h sgxmem a) =
+    (forall (h0:sgxmem) (b:bool). wp (fun r b -> True) h0 b)
 
 new_effect {
-  STX_h (heap:Type) : a:Type -> wp:est_wp_h heap a -> Effect
+  STX_h (sgxmem:Type) : a:Type -> wp:stx_wp_h sgxmem a -> Effect
   with
-    return_wp    = stx_return       heap
-  ; bind_wp      = stx_bind_wp      heap
-  ; if_then_else = stx_if_then_else heap
-  ; ite_wp       = stx_ite_wp       heap
-  ; stronger     = stx_stronger     heap
-  ; close_wp     = stx_close_wp     heap
-  ; assert_p     = stx_assert_p     heap
-  ; assume_p     = stx_assume_p     heap
-  ; null_wp      = stx_null_wp      heap
-  ; trivial      = stx_trivial      heap
+    return_wp    = stx_return       sgxmem
+  ; bind_wp      = stx_bind_wp      sgxmem
+  ; if_then_else = stx_if_then_else sgxmem
+  ; ite_wp       = stx_ite_wp       sgxmem
+  ; stronger     = stx_stronger     sgxmem
+  ; close_wp     = stx_close_wp     sgxmem
+  ; assert_p     = stx_assert_p     sgxmem
+  ; assume_p     = stx_assume_p     sgxmem
+  ; null_wp      = stx_null_wp      sgxmem
+  ; trivial      = stx_trivial      sgxmem
 }
 (* </skip> until here *)
 ////////////////////////////////////////////////////////////////////////////////
-open FStar.Heap 
-new_effect STX = STX_h heap //Define a instance of ES, specializing the memory to heaps
 
-(* Eth is our effect, in Hoare triple style with pre-conditions and post-conditions *)
-effect Eth (a:Type) 
-	   (pre:heap -> bool -> Type0)
-	   (post:heap -> bool -> option (a * heap) -> bool -> Type0)
-       = STX a (fun (q:option (a * heap) -> bool -> Type0) (h0:heap) (b0:bool) -> 
+open FStar.SGX
+
+new_effect STX = STX_h sgxmem //Define a instance of STX_h, specializing the memory to sgxmem
+
+(* Sth is our effect, in Hoare triple style with pre-conditions and post-conditions *)
+effect Sth (a:Type) 
+	   (pre:sgxmem -> bool -> Type0)
+	   (post:sgxmem -> bool -> option (a * sgxmem) -> bool -> Type0)
+       = STX a (fun (q:option (a * sgxmem) -> bool -> Type0) (h0:sgxmem) (b0:bool) -> 
 		  pre h0 b0
 		  /\ (forall r b1. post h0 b0 r b1 ==> q r b1))
 	 
 
-(* operations for STX *)
-(* This is my best guess so far at the desired semantics of the operations.
-   We should discuss further to see if that matches reality *)
-assume val throw : unit -> Eth unit 
+(* operations for STX. In Progress *)
+assume val throw : unit -> Sth unit 
   (requires (fun _ _ -> True))
   (ensures (fun h0 b0 r b1 -> b0=b1 /\ r==None)) //state is reset; flag doesn't change
 
-assume val send: msg:nat -> Eth bool
-  (requires (fun _ b0 -> not b0))      //can only send if we are not already in a "failed send" state
+assume val write: addr:sgxref a->value:nat -> Sth bool
+  (requires (fun h0 b0 -> not b0 /\ 		//can only write if we are not already in a "failed read/write" state 
+		isbitmapset h0 addr))		//and if the corresponding address is protected in bitmap 
   (ensures (fun h0 b0 r b1 -> 
-		 r==Some (b1, h0))) //the return value is the flag and the heap doesn't change
+		 r==Some (b1, h0))) //the return value is the flag and the modified heap. FIXME: How to return modified heap 
 
-assume val alloc:  #a:Type -> init:a -> Eth (ref a)
+assume val read:  #a:Type -> x:ref a -> Sth a
+   (requires (fun _ b0 -> not b0 		//can only read if we are not already in a "failed read/write" state
+		isbitmapset h0 addr))		//and if the corresponding address is protected in bitmap 
+   (ensures (fun h0 b0 r b1 -> 
+	       r==Some (sel h0 x, h0)))
+
+assume val alloc:  #a:Type -> init:a -> Sth (ref a)
   (requires (fun _ _ -> True)) //allocation effects are always permitted
   (ensures (fun h0 b0 r b1 -> 
 	      b0=b1 /\ //the flag doesn't change
@@ -137,17 +135,5 @@ assume val alloc:  #a:Type -> init:a -> Eth (ref a)
 	       | Some (x, h1) -> 
 	  	  not(contains h0 x)  //the returned ref is fresh
 		/\ contains h1 x
-		/\ h1==upd h0 x init))) //and the heap is updated appropriately
-
-assume val recall:  #a:Type -> x:ref a -> Eth unit
-   (requires (fun h0 b0 -> True)) 
-   (ensures (fun h0 b0 r b1 ->  r == Some ((), h0)
-			  /\ b0 = b1
-			  /\ Heap.contains h0 x))
-
-assume val read:  #a:Type -> x:ref a -> Eth a
-   (requires (fun _ _ -> True)) //read effects are always permitted
-   (ensures (fun h0 b0 r b1 -> 
-	       b0=b1 /\ //the flag doesn't change
-	       r==Some (sel h0 x, h0)))
+		/\ h1==upd h0 x init))) //and the sgxmem is updated appropriately
 
